misc tuning and modernization;

src/HOL/Hilbert_Choice.thy
@@ -6,23 +6,23 @@
 section \<open>Hilbert's Epsilon-Operator and the Axiom of Choice\<close>
 
 theory Hilbert_Choice
-imports Wellfounded
-keywords "specification" :: thy_goal
+  imports Wellfounded
+  keywords "specification" :: thy_goal
 begin
 
 subsection \<open>Hilbert's epsilon\<close>
 
-axiomatization Eps :: "('a => bool) => 'a" where
-  someI: "P x ==> P (Eps P)"
+axiomatization Eps :: "('a \<Rightarrow> bool) \<Rightarrow> 'a"
+  where someI: "P x \<Longrightarrow> P (Eps P)"
 
 syntax (epsilon)
-  "_Eps"        :: "[pttrn, bool] => 'a"    ("(3\<some>_./ _)" [0, 10] 10)
+  "_Eps" :: "pttrn \<Rightarrow> bool \<Rightarrow> 'a"  ("(3\<some>_./ _)" [0, 10] 10)
 syntax (input)
-  "_Eps"        :: "[pttrn, bool] => 'a"    ("(3@ _./ _)" [0, 10] 10)
+  "_Eps" :: "pttrn \<Rightarrow> bool \<Rightarrow> 'a"  ("(3@ _./ _)" [0, 10] 10)
 syntax
-  "_Eps"        :: "[pttrn, bool] => 'a"    ("(3SOME _./ _)" [0, 10] 10)
+  "_Eps" :: "pttrn \<Rightarrow> bool \<Rightarrow> 'a"  ("(3SOME _./ _)" [0, 10] 10)
 translations
-  "SOME x. P" == "CONST Eps (%x. P)"
+  "SOME x. P" \<rightleftharpoons> "CONST Eps (\<lambda>x. P)"
 
 print_translation \<open>
   [(@{const_syntax Eps}, fn _ => fn [Abs abs] =>
@@ -30,90 +30,92 @@ print_translation \<open>
       in Syntax.const @{syntax_const "_Eps"} $ x $ t end)]
 \<close> \<comment> \<open>to avoid eta-contraction of body\<close>
 
-definition inv_into :: "'a set => ('a => 'b) => ('b => 'a)" where
-"inv_into A f == %x. SOME y. y : A & f y = x"
+definition inv_into :: "'a set \<Rightarrow> ('a \<Rightarrow> 'b) \<Rightarrow> ('b \<Rightarrow> 'a)"
+  where "inv_into A f \<equiv> \<lambda>x. SOME y. y \<in> A \<and> f y = x"
 
-abbreviation inv :: "('a => 'b) => ('b => 'a)" where
-"inv == inv_into UNIV"
+abbreviation inv :: "('a \<Rightarrow> 'b) \<Rightarrow> ('b \<Rightarrow> 'a)"
+  where "inv \<equiv> inv_into UNIV"
 
 
 subsection \<open>Hilbert's Epsilon-operator\<close>
 
-text\<open>Easier to apply than \<open>someI\<close> if the witness comes from an
-existential formula\<close>
-lemma someI_ex [elim?]: "\<exists>x. P x ==> P (SOME x. P x)"
-apply (erule exE)
-apply (erule someI)
-done
+text \<open>
+  Easier to apply than \<open>someI\<close> if the witness comes from an
+  existential formula.
+\<close>
+lemma someI_ex [elim?]: "\<exists>x. P x \<Longrightarrow> P (SOME x. P x)"
+  apply (erule exE)
+  apply (erule someI)
+  done
 
-text\<open>Easier to apply than \<open>someI\<close> because the conclusion has only one
-occurrence of @{term P}.\<close>
-lemma someI2: "[| P a;  !!x. P x ==> Q x |] ==> Q (SOME x. P x)"
+text \<open>
+  Easier to apply than \<open>someI\<close> because the conclusion has only one
+  occurrence of @{term P}.
+\<close>
+lemma someI2: "P a \<Longrightarrow> (\<And>x. P x \<Longrightarrow> Q x) \<Longrightarrow> Q (SOME x. P x)"
   by (blast intro: someI)
 
-text\<open>Easier to apply than \<open>someI2\<close> if the witness comes from an
-existential formula\<close>
-
-lemma someI2_ex: "[| \<exists>a. P a; !!x. P x ==> Q x |] ==> Q (SOME x. P x)"
+text \<open>
+  Easier to apply than \<open>someI2\<close> if the witness comes from an
+  existential formula.
+\<close>
+lemma someI2_ex: "\<exists>a. P a \<Longrightarrow> (\<And>x. P x \<Longrightarrow> Q x) \<Longrightarrow> Q (SOME x. P x)"
   by (blast intro: someI2)
 
-lemma someI2_bex: "[| \<exists>a\<in>A. P a; !!x. x \<in> A \<and> P x ==> Q x |] ==> Q (SOME x. x \<in> A \<and> P x)"
+lemma someI2_bex: "\<exists>a\<in>A. P a \<Longrightarrow> (\<And>x. x \<in> A \<and> P x \<Longrightarrow> Q x) \<Longrightarrow> Q (SOME x. x \<in> A \<and> P x)"
   by (blast intro: someI2)
 
-lemma some_equality [intro]:
-     "[| P a;  !!x. P x ==> x=a |] ==> (SOME x. P x) = a"
-by (blast intro: someI2)
+lemma some_equality [intro]: "P a \<Longrightarrow> (\<And>x. P x \<Longrightarrow> x = a) \<Longrightarrow> (SOME x. P x) = a"
+  by (blast intro: someI2)
 
-lemma some1_equality: "[| EX!x. P x; P a |] ==> (SOME x. P x) = a"
-by blast
+lemma some1_equality: "EX!x. P x \<Longrightarrow> P a \<Longrightarrow> (SOME x. P x) = a"
+  by blast
 
-lemma some_eq_ex: "P (SOME x. P x) =  (\<exists>x. P x)"
-by (blast intro: someI)
+lemma some_eq_ex: "P (SOME x. P x) \<longleftrightarrow> (\<exists>x. P x)"
+  by (blast intro: someI)
 
 lemma some_in_eq: "(SOME x. x \<in> A) \<in> A \<longleftrightarrow> A \<noteq> {}"
   unfolding ex_in_conv[symmetric] by (rule some_eq_ex)
 
-lemma some_eq_trivial [simp]: "(SOME y. y=x) = x"
-apply (rule some_equality)
-apply (rule refl, assumption)
-done
+lemma some_eq_trivial [simp]: "(SOME y. y = x) = x"
+  by (rule some_equality) (rule refl)
 
-lemma some_sym_eq_trivial [simp]: "(SOME y. x=y) = x"
-apply (rule some_equality)
-apply (rule refl)
-apply (erule sym)
-done
+lemma some_sym_eq_trivial [simp]: "(SOME y. x = y) = x"
+  apply (rule some_equality)
+   apply (rule refl)
+  apply (erule sym)
+  done
 
 
-subsection\<open>Axiom of Choice, Proved Using the Description Operator\<close>
+subsection \<open>Axiom of Choice, Proved Using the Description Operator\<close>
 
-lemma choice: "\<forall>x. \<exists>y. Q x y ==> \<exists>f. \<forall>x. Q x (f x)"
-by (fast elim: someI)
+lemma choice: "\<forall>x. \<exists>y. Q x y \<Longrightarrow> \<exists>f. \<forall>x. Q x (f x)"
+  by (fast elim: someI)
 
-lemma bchoice: "\<forall>x\<in>S. \<exists>y. Q x y ==> \<exists>f. \<forall>x\<in>S. Q x (f x)"
-by (fast elim: someI)
+lemma bchoice: "\<forall>x\<in>S. \<exists>y. Q x y \<Longrightarrow> \<exists>f. \<forall>x\<in>S. Q x (f x)"
+  by (fast elim: someI)
 
 lemma choice_iff: "(\<forall>x. \<exists>y. Q x y) \<longleftrightarrow> (\<exists>f. \<forall>x. Q x (f x))"
-by (fast elim: someI)
+  by (fast elim: someI)
 
 lemma choice_iff': "(\<forall>x. P x \<longrightarrow> (\<exists>y. Q x y)) \<longleftrightarrow> (\<exists>f. \<forall>x. P x \<longrightarrow> Q x (f x))"
-by (fast elim: someI)
+  by (fast elim: someI)
 
 lemma bchoice_iff: "(\<forall>x\<in>S. \<exists>y. Q x y) \<longleftrightarrow> (\<exists>f. \<forall>x\<in>S. Q x (f x))"
-by (fast elim: someI)
+  by (fast elim: someI)
 
 lemma bchoice_iff': "(\<forall>x\<in>S. P x \<longrightarrow> (\<exists>y. Q x y)) \<longleftrightarrow> (\<exists>f. \<forall>x\<in>S. P x \<longrightarrow> Q x (f x))"
-by (fast elim: someI)
+  by (fast elim: someI)
 
 lemma dependent_nat_choice:
-  assumes  1: "\<exists>x. P 0 x" and
-           2: "\<And>x n. P n x \<Longrightarrow> \<exists>y. P (Suc n) y \<and> Q n x y"
+  assumes 1: "\<exists>x. P 0 x"
+    and 2: "\<And>x n. P n x \<Longrightarrow> \<exists>y. P (Suc n) y \<and> Q n x y"
   shows "\<exists>f. \<forall>n. P n (f n) \<and> Q n (f n) (f (Suc n))"
 proof (intro exI allI conjI)
   fix n
   define f where "f = rec_nat (SOME x. P 0 x) (\<lambda>n x. SOME y. P (Suc n) y \<and> Q n x y)"
-  have "P 0 (f 0)" "\<And>n. P n (f n) \<Longrightarrow> P (Suc n) (f (Suc n)) \<and> Q n (f n) (f (Suc n))"
-    using someI_ex[OF 1] someI_ex[OF 2] by (simp_all add: f_def)
+  then have "P 0 (f 0)" "\<And>n. P n (f n) \<Longrightarrow> P (Suc n) (f (Suc n)) \<and> Q n (f n) (f (Suc n))"
+    using someI_ex[OF 1] someI_ex[OF 2] by simp_all
   then show "P n (f n)" "Q n (f n) (f (Suc n))"
     by (induct n) auto
 qed
@@ -121,181 +123,172 @@ qed
 
 subsection \<open>Function Inverse\<close>
 
-lemma inv_def: "inv f = (%y. SOME x. f x = y)"
-by(simp add: inv_into_def)
+lemma inv_def: "inv f = (\<lambda>y. SOME x. f x = y)"
+  by (simp add: inv_into_def)
 
-lemma inv_into_into: "x : f ` A ==> inv_into A f x : A"
-apply (simp add: inv_into_def)
-apply (fast intro: someI2)
-done
+lemma inv_into_into: "x \<in> f ` A \<Longrightarrow> inv_into A f x \<in> A"
+  by (simp add: inv_into_def) (fast intro: someI2)
 
-lemma inv_identity [simp]:
-  "inv (\<lambda>a. a) = (\<lambda>a. a)"
+lemma inv_identity [simp]: "inv (\<lambda>a. a) = (\<lambda>a. a)"
   by (simp add: inv_def)
 
-lemma inv_id [simp]:
-  "inv id = id"
+lemma inv_id [simp]: "inv id = id"
   by (simp add: id_def)
 
-lemma inv_into_f_f [simp]:
-  "[| inj_on f A;  x : A |] ==> inv_into A f (f x) = x"
-apply (simp add: inv_into_def inj_on_def)
-apply (blast intro: someI2)
-done
+lemma inv_into_f_f [simp]: "inj_on f A \<Longrightarrow> x \<in> A \<Longrightarrow> inv_into A f (f x) = x"
+  by (simp add: inv_into_def inj_on_def) (blast intro: someI2)
 
-lemma inv_f_f: "inj f ==> inv f (f x) = x"
-by simp
+lemma inv_f_f: "inj f \<Longrightarrow> inv f (f x) = x"
+  by simp
 
-lemma f_inv_into_f: "y : f`A  ==> f (inv_into A f y) = y"
-apply (simp add: inv_into_def)
-apply (fast intro: someI2)
-done
+lemma f_inv_into_f: "y : f`A \<Longrightarrow> f (inv_into A f y) = y"
+  by (simp add: inv_into_def) (fast intro: someI2)
 
-lemma inv_into_f_eq: "[| inj_on f A; x : A; f x = y |] ==> inv_into A f y = x"
-apply (erule subst)
-apply (fast intro: inv_into_f_f)
-done
+lemma inv_into_f_eq: "inj_on f A \<Longrightarrow> x \<in> A \<Longrightarrow> f x = y \<Longrightarrow> inv_into A f y = x"
+  by (erule subst) (fast intro: inv_into_f_f)
 
-lemma inv_f_eq: "[| inj f; f x = y |] ==> inv f y = x"
-by (simp add:inv_into_f_eq)
+lemma inv_f_eq: "inj f \<Longrightarrow> f x = y \<Longrightarrow> inv f y = x"
+  by (simp add:inv_into_f_eq)
 
-lemma inj_imp_inv_eq: "[| inj f; ALL x. f(g x) = x |] ==> inv f = g"
+lemma inj_imp_inv_eq: "inj f \<Longrightarrow> \<forall>x. f (g x) = x \<Longrightarrow> inv f = g"
   by (blast intro: inv_into_f_eq)
 
-text\<open>But is it useful?\<close>
+text \<open>But is it useful?\<close>
 lemma inj_transfer:
-  assumes injf: "inj f" and minor: "!!y. y \<in> range(f) ==> P(inv f y)"
+  assumes inj: "inj f"
+    and minor: "\<And>y. y \<in> range f \<Longrightarrow> P (inv f y)"
   shows "P x"
 proof -
   have "f x \<in> range f" by auto
-  hence "P(inv f (f x))" by (rule minor)
-  thus "P x" by (simp add: inv_into_f_f [OF injf])
+  then have "P(inv f (f x))" by (rule minor)
+  then show "P x" by (simp add: inv_into_f_f [OF inj])
 qed
 
-lemma inj_iff: "(inj f) = (inv f o f = id)"
-apply (simp add: o_def fun_eq_iff)
-apply (blast intro: inj_on_inverseI inv_into_f_f)
-done
+lemma inj_iff: "inj f \<longleftrightarrow> inv f \<circ> f = id"
+  by (simp add: o_def fun_eq_iff) (blast intro: inj_on_inverseI inv_into_f_f)
 
-lemma inv_o_cancel[simp]: "inj f ==> inv f o f = id"
-by (simp add: inj_iff)
+lemma inv_o_cancel[simp]: "inj f \<Longrightarrow> inv f \<circ> f = id"
+  by (simp add: inj_iff)
 
-lemma o_inv_o_cancel[simp]: "inj f ==> g o inv f o f = g"
-by (simp add: comp_assoc)
+lemma o_inv_o_cancel[simp]: "inj f \<Longrightarrow> g \<circ> inv f \<circ> f = g"
+  by (simp add: comp_assoc)
 
-lemma inv_into_image_cancel[simp]:
-  "inj_on f A ==> S <= A ==> inv_into A f ` f ` S = S"
-by(fastforce simp: image_def)
+lemma inv_into_image_cancel[simp]: "inj_on f A \<Longrightarrow> S \<subseteq> A \<Longrightarrow> inv_into A f ` f ` S = S"
+  by (fastforce simp: image_def)
 
-lemma inj_imp_surj_inv: "inj f ==> surj (inv f)"
-by (blast intro!: surjI inv_into_f_f)
+lemma inj_imp_surj_inv: "inj f \<Longrightarrow> surj (inv f)"
+  by (blast intro!: surjI inv_into_f_f)
 
-lemma surj_f_inv_f: "surj f ==> f(inv f y) = y"
-by (simp add: f_inv_into_f)
+lemma surj_f_inv_f: "surj f \<Longrightarrow> f (inv f y) = y"
+  by (simp add: f_inv_into_f)
 
 lemma inv_into_injective:
   assumes eq: "inv_into A f x = inv_into A f y"
-      and x: "x: f`A"
-      and y: "y: f`A"
-  shows "x=y"
+    and x: "x \<in> f`A"
+    and y: "y \<in> f`A"
+  shows "x = y"
 proof -
-  have "f (inv_into A f x) = f (inv_into A f y)" using eq by simp
-  thus ?thesis by (simp add: f_inv_into_f x y)
+  from eq have "f (inv_into A f x) = f (inv_into A f y)"
+    by simp
+  with x y show ?thesis
+    by (simp add: f_inv_into_f)
 qed
 
-lemma inj_on_inv_into: "B <= f`A ==> inj_on (inv_into A f) B"
-by (blast intro: inj_onI dest: inv_into_injective injD)
+lemma inj_on_inv_into: "B \<subseteq> f`A \<Longrightarrow> inj_on (inv_into A f) B"
+  by (blast intro: inj_onI dest: inv_into_injective injD)
 
-lemma bij_betw_inv_into: "bij_betw f A B ==> bij_betw (inv_into A f) B A"
-by (auto simp add: bij_betw_def inj_on_inv_into)
+lemma bij_betw_inv_into: "bij_betw f A B \<Longrightarrow> bij_betw (inv_into A f) B A"
+  by (auto simp add: bij_betw_def inj_on_inv_into)
 
-lemma surj_imp_inj_inv: "surj f ==> inj (inv f)"
-by (simp add: inj_on_inv_into)
+lemma surj_imp_inj_inv: "surj f \<Longrightarrow> inj (inv f)"
+  by (simp add: inj_on_inv_into)
 
-lemma surj_iff: "(surj f) = (f o inv f = id)"
-by (auto intro!: surjI simp: surj_f_inv_f fun_eq_iff[where 'b='a])
+lemma surj_iff: "surj f \<longleftrightarrow> f \<circ> inv f = id"
+  by (auto intro!: surjI simp: surj_f_inv_f fun_eq_iff[where 'b='a])
 
 lemma surj_iff_all: "surj f \<longleftrightarrow> (\<forall>x. f (inv f x) = x)"
-  unfolding surj_iff by (simp add: o_def fun_eq_iff)
+  by (simp add: o_def surj_iff fun_eq_iff)
 
-lemma surj_imp_inv_eq: "[| surj f; \<forall>x. g(f x) = x |] ==> inv f = g"
-apply (rule ext)
-apply (drule_tac x = "inv f x" in spec)
-apply (simp add: surj_f_inv_f)
-done
+lemma surj_imp_inv_eq: "surj f \<Longrightarrow> \<forall>x. g (f x) = x \<Longrightarrow> inv f = g"
+  apply (rule ext)
+  apply (drule_tac x = "inv f x" in spec)
+  apply (simp add: surj_f_inv_f)
+  done
 
-lemma bij_imp_bij_inv: "bij f ==> bij (inv f)"
-by (simp add: bij_def inj_imp_surj_inv surj_imp_inj_inv)
+lemma bij_imp_bij_inv: "bij f \<Longrightarrow> bij (inv f)"
+  by (simp add: bij_def inj_imp_surj_inv surj_imp_inj_inv)
 
-lemma inv_equality: "[| !!x. g (f x) = x;  !!y. f (g y) = y |] ==> inv f = g"
-apply (rule ext)
-apply (auto simp add: inv_into_def)
-done
+lemma inv_equality: "(\<And>x. g (f x) = x) \<Longrightarrow> (\<And>y. f (g y) = y) \<Longrightarrow> inv f = g"
+  by (rule ext) (auto simp add: inv_into_def)
 
-lemma inv_inv_eq: "bij f ==> inv (inv f) = f"
-apply (rule inv_equality)
-apply (auto simp add: bij_def surj_f_inv_f)
-done
+lemma inv_inv_eq: "bij f \<Longrightarrow> inv (inv f) = f"
+  by (rule inv_equality) (auto simp add: bij_def surj_f_inv_f)
 
-(** bij(inv f) implies little about f.  Consider f::bool=>bool such that
-    f(True)=f(False)=True.  Then it's consistent with axiom someI that
-    inv f could be any function at all, including the identity function.
-    If inv f=id then inv f is a bijection, but inj f, surj(f) and
-    inv(inv f)=f all fail.
-**)
+text \<open>
+  \<open>bij (inv f)\<close> implies little about \<open>f\<close>. Consider \<open>f :: bool \<Rightarrow> bool\<close> such
+  that \<open>f True = f False = True\<close>. Then it ia consistent with axiom \<open>someI\<close>
+  that \<open>inv f\<close> could be any function at all, including the identity function.
+  If \<open>inv f = id\<close> then \<open>inv f\<close> is a bijection, but \<open>inj f\<close>, \<open>surj f\<close> and \<open>inv
+  (inv f) = f\<close> all fail.
+\<close>
 
 lemma inv_into_comp:
-  "[| inj_on f (g ` A); inj_on g A; x : f ` g ` A |] ==>
-  inv_into A (f o g) x = (inv_into A g o inv_into (g ` A) f) x"
-apply (rule inv_into_f_eq)
-  apply (fast intro: comp_inj_on)
- apply (simp add: inv_into_into)
-apply (simp add: f_inv_into_f inv_into_into)
-done
+  "inj_on f (g ` A) \<Longrightarrow> inj_on g A \<Longrightarrow> x \<in> f ` g ` A \<Longrightarrow>
+    inv_into A (f \<circ> g) x = (inv_into A g \<circ> inv_into (g ` A) f) x"
+  apply (rule inv_into_f_eq)
+    apply (fast intro: comp_inj_on)
+   apply (simp add: inv_into_into)
+  apply (simp add: f_inv_into_f inv_into_into)
+  done
 
-lemma o_inv_distrib: "[| bij f; bij g |] ==> inv (f o g) = inv g o inv f"
-apply (rule inv_equality)
-apply (auto simp add: bij_def surj_f_inv_f)
-done
+lemma o_inv_distrib: "bij f \<Longrightarrow> bij g \<Longrightarrow> inv (f \<circ> g) = inv g \<circ> inv f"
+  by (rule inv_equality) (auto simp add: bij_def surj_f_inv_f)
 
-lemma image_surj_f_inv_f: "surj f ==> f ` (inv f ` A) = A"
+lemma image_surj_f_inv_f: "surj f \<Longrightarrow> f ` (inv f ` A) = A"
   by (simp add: surj_f_inv_f image_comp comp_def)
 
-lemma image_inv_f_f: "inj f ==> inv f ` (f ` A) = A"
+lemma image_inv_f_f: "inj f \<Longrightarrow> inv f ` (f ` A) = A"
   by simp
 
-lemma inv_image_comp: "inj f ==> inv f ` (f ` X) = X"
+lemma inv_image_comp: "inj f \<Longrightarrow> inv f ` (f ` X) = X"
   by (fact image_inv_f_f)
 
-lemma bij_image_Collect_eq: "bij f ==> f ` Collect P = {y. P (inv f y)}"
-apply auto
-apply (force simp add: bij_is_inj)
-apply (blast intro: bij_is_surj [THEN surj_f_inv_f, symmetric])
-done
+lemma bij_image_Collect_eq: "bij f \<Longrightarrow> f ` Collect P = {y. P (inv f y)}"
+  apply auto
+   apply (force simp add: bij_is_inj)
+  apply (blast intro: bij_is_surj [THEN surj_f_inv_f, symmetric])
+  done
 
-lemma bij_vimage_eq_inv_image: "bij f ==> f -` A = inv f ` A"
-apply (auto simp add: bij_is_surj [THEN surj_f_inv_f])
-apply (blast intro: bij_is_inj [THEN inv_into_f_f, symmetric])
-done
+lemma bij_vimage_eq_inv_image: "bij f \<Longrightarrow> f -` A = inv f ` A"
+  apply (auto simp add: bij_is_surj [THEN surj_f_inv_f])
+  apply (blast intro: bij_is_inj [THEN inv_into_f_f, symmetric])
+  done
 
 lemma finite_fun_UNIVD1:
   assumes fin: "finite (UNIV :: ('a \<Rightarrow> 'b) set)"
-  and card: "card (UNIV :: 'b set) \<noteq> Suc 0"
+    and card: "card (UNIV :: 'b set) \<noteq> Suc 0"
   shows "finite (UNIV :: 'a set)"
 proof -
-  from fin have finb: "finite (UNIV :: 'b set)" by (rule finite_fun_UNIVD2)
+  from fin have finb: "finite (UNIV :: 'b set)"
+    by (rule finite_fun_UNIVD2)
   with card have "card (UNIV :: 'b set) \<ge> Suc (Suc 0)"
     by (cases "card (UNIV :: 'b set)") (auto simp add: card_eq_0_iff)
-  then obtain n where "card (UNIV :: 'b set) = Suc (Suc n)" "n = card (UNIV :: 'b set) - Suc (Suc 0)" by auto
-  then obtain b1 b2 where b1b2: "(b1 :: 'b) \<noteq> (b2 :: 'b)" by (auto simp add: card_Suc_eq)
-  from fin have "finite (range (\<lambda>f :: 'a \<Rightarrow> 'b. inv f b1))" by (rule finite_imageI)
+  then obtain n where "card (UNIV :: 'b set) = Suc (Suc n)" "n = card (UNIV :: 'b set) - Suc (Suc 0)"
+    by auto
+  then obtain b1 b2 where b1b2: "(b1 :: 'b) \<noteq> (b2 :: 'b)"
+    by (auto simp add: card_Suc_eq)
+  from fin have "finite (range (\<lambda>f :: 'a \<Rightarrow> 'b. inv f b1))"
+    by (rule finite_imageI)
   moreover have "UNIV = range (\<lambda>f :: 'a \<Rightarrow> 'b. inv f b1)"
   proof (rule UNIV_eq_I)
     fix x :: 'a
-    from b1b2 have "x = inv (\<lambda>y. if y = x then b1 else b2) b1" by (simp add: inv_into_def)
-    thus "x \<in> range (\<lambda>f::'a \<Rightarrow> 'b. inv f b1)" by blast
+    from b1b2 have "x = inv (\<lambda>y. if y = x then b1 else b2) b1"
+      by (simp add: inv_into_def)
+    then show "x \<in> range (\<lambda>f::'a \<Rightarrow> 'b. inv f b1)"
+      by blast
   qed
-  ultimately show "finite (UNIV :: 'a set)" by simp
+  ultimately show "finite (UNIV :: 'a set)"
+    by simp
 qed
 
 text \<open>
@@ -318,18 +311,18 @@ proof -
   define Sseq where "Sseq = rec_nat S (\<lambda>n T. T - {SOME e. e \<in> T})"
   define pick where "pick n = (SOME e. e \<in> Sseq n)" for n
   have *: "Sseq n \<subseteq> S" "\<not> finite (Sseq n)" for n
-    by (induct n) (auto simp add: Sseq_def inf)
+    by (induct n) (auto simp: Sseq_def inf)
   then have **: "\<And>n. pick n \<in> Sseq n"
     unfolding pick_def by (subst (asm) finite.simps) (auto simp add: ex_in_conv intro: someI_ex)
   with * have "range pick \<subseteq> S" by auto
-  moreover
-  {
-    fix n m
+  moreover have "pick n \<noteq> pick (n + Suc m)" for m n
+  proof -
     have "pick n \<notin> Sseq (n + Suc m)"
       by (induct m) (auto simp add: Sseq_def pick_def)
-    with ** have "pick n \<noteq> pick (n + Suc m)" by auto
-  }
-  then have "inj pick" by (intro linorder_injI) (auto simp add: less_iff_Suc_add)
+    with ** show ?thesis by auto
+  qed
+  then have "inj pick"
+    by (intro linorder_injI) (auto simp add: less_iff_Suc_add)
   ultimately show ?thesis by blast
 qed
 
@@ -338,31 +331,35 @@ lemma infinite_iff_countable_subset: "\<not> finite S \<longleftrightarrow> (\<e
   using finite_imageD finite_subset infinite_UNIV_char_0 infinite_countable_subset by auto
 
 lemma image_inv_into_cancel:
-  assumes SURJ: "f`A=A'" and SUB: "B' \<le> A'"
+  assumes surj: "f`A = A'"
+    and sub: "B' \<subseteq> A'"
   shows "f `((inv_into A f)`B') = B'"
   using assms
-proof (auto simp add: f_inv_into_f)
-  let ?f' = "(inv_into A f)"
-  fix a' assume *: "a' \<in> B'"
-  then have "a' \<in> A'" using SUB by auto
-  then have "a' = f (?f' a')"
-    using SURJ by (auto simp add: f_inv_into_f)
-  then show "a' \<in> f ` (?f' ` B')" using * by blast
+proof (auto simp: f_inv_into_f)
+  let ?f' = "inv_into A f"
+  fix a'
+  assume *: "a' \<in> B'"
+  with sub have "a' \<in> A'" by auto
+  with surj have "a' = f (?f' a')"
+    by (auto simp: f_inv_into_f)
+  with * show "a' \<in> f ` (?f' ` B')" by blast
 qed
 
 lemma inv_into_inv_into_eq:
-  assumes "bij_betw f A A'" "a \<in> A"
+  assumes "bij_betw f A A'"
+    and a: "a \<in> A"
   shows "inv_into A' (inv_into A f) a = f a"
 proof -
-  let ?f' = "inv_into A f"   let ?f'' = "inv_into A' ?f'"
-  have 1: "bij_betw ?f' A' A" using assms
-  by (auto simp add: bij_betw_inv_into)
-  obtain a' where 2: "a' \<in> A'" and 3: "?f' a' = a"
-    using 1 \<open>a \<in> A\<close> unfolding bij_betw_def by force
-  hence "?f'' a = a'"
-    using \<open>a \<in> A\<close> 1 3 by (auto simp add: f_inv_into_f bij_betw_def)
-  moreover have "f a = a'" using assms 2 3
-    by (auto simp add: bij_betw_def)
+  let ?f' = "inv_into A f"
+  let ?f'' = "inv_into A' ?f'"
+  from assms have *: "bij_betw ?f' A' A"
+    by (auto simp: bij_betw_inv_into)
+  with a obtain a' where a': "a' \<in> A'" "?f' a' = a"
+    unfolding bij_betw_def by force
+  with a * have "?f'' a = a'"
+    by (auto simp: f_inv_into_f bij_betw_def)
+  moreover from assms a' have "f a = a'"
+    by (auto simp: bij_betw_def)
   ultimately show "?f'' a = f a" by simp
 qed
 
@@ -370,72 +367,82 @@ lemma inj_on_iff_surj:
   assumes "A \<noteq> {}"
   shows "(\<exists>f. inj_on f A \<and> f ` A \<le> A') \<longleftrightarrow> (\<exists>g. g ` A' = A)"
 proof safe
-  fix f assume INJ: "inj_on f A" and INCL: "f ` A \<le> A'"
-  let ?phi = "\<lambda>a' a. a \<in> A \<and> f a = a'"  let ?csi = "\<lambda>a. a \<in> A"
+  fix f
+  assume inj: "inj_on f A" and incl: "f ` A \<subseteq> A'"
+  let ?phi = "\<lambda>a' a. a \<in> A \<and> f a = a'"
+  let ?csi = "\<lambda>a. a \<in> A"
   let ?g = "\<lambda>a'. if a' \<in> f ` A then (SOME a. ?phi a' a) else (SOME a. ?csi a)"
   have "?g ` A' = A"
   proof
-    show "?g ` A' \<le> A"
+    show "?g ` A' \<subseteq> A"
     proof clarify
-      fix a' assume *: "a' \<in> A'"
+      fix a'
+      assume *: "a' \<in> A'"
       show "?g a' \<in> A"
-      proof cases
-        assume Case1: "a' \<in> f ` A"
+      proof (cases "a' \<in> f ` A")
+        case True
         then obtain a where "?phi a' a" by blast
-        hence "?phi a' (SOME a. ?phi a' a)" using someI[of "?phi a'" a] by blast
-        with Case1 show ?thesis by auto
+        then have "?phi a' (SOME a. ?phi a' a)"
+          using someI[of "?phi a'" a] by blast
+        with True show ?thesis by auto
       next
-        assume Case2: "a' \<notin> f ` A"
-        hence "?csi (SOME a. ?csi a)" using assms someI_ex[of ?csi] by blast
-        with Case2 show ?thesis by auto
+        case False
+        with assms have "?csi (SOME a. ?csi a)"
+          using someI_ex[of ?csi] by blast
+        with False show ?thesis by auto
       qed
     qed
   next
-    show "A \<le> ?g ` A'"
-    proof-
-      {fix a assume *: "a \<in> A"
-       let ?b = "SOME aa. ?phi (f a) aa"
-       have "?phi (f a) a" using * by auto
-       hence 1: "?phi (f a) ?b" using someI[of "?phi(f a)" a] by blast
-       hence "?g(f a) = ?b" using * by auto
-       moreover have "a = ?b" using 1 INJ * by (auto simp add: inj_on_def)
-       ultimately have "?g(f a) = a" by simp
-       with INCL * have "?g(f a) = a \<and> f a \<in> A'" by auto
-      }
-      thus ?thesis by force
+    show "A \<subseteq> ?g ` A'"
+    proof -
+      have "?g (f a) = a \<and> f a \<in> A'" if a: "a \<in> A" for a
+      proof -
+        let ?b = "SOME aa. ?phi (f a) aa"
+        from a have "?phi (f a) a" by auto
+        then have *: "?phi (f a) ?b"
+          using someI[of "?phi(f a)" a] by blast
+        then have "?g (f a) = ?b" using a by auto
+        moreover from inj * a have "a = ?b"
+          by (auto simp add: inj_on_def)
+        ultimately have "?g(f a) = a" by simp
+        with incl a show ?thesis by auto
+      qed
+      then show ?thesis by force
     qed
   qed
-  thus "\<exists>g. g ` A' = A" by blast
+  then show "\<exists>g. g ` A' = A" by blast
 next
-  fix g  let ?f = "inv_into A' g"
+  fix g
+  let ?f = "inv_into A' g"
   have "inj_on ?f (g ` A')"
-    by (auto simp add: inj_on_inv_into)
-  moreover
-  {fix a' assume *: "a' \<in> A'"
-   let ?phi = "\<lambda> b'. b' \<in> A' \<and> g b' = g a'"
-   have "?phi a'" using * by auto
-   hence "?phi(SOME b'. ?phi b')" using someI[of ?phi] by blast
-   hence "?f(g a') \<in> A'" unfolding inv_into_def by auto
-  }
-  ultimately show "\<exists>f. inj_on f (g ` A') \<and> f ` g ` A' \<subseteq> A'" by auto
+    by (auto simp: inj_on_inv_into)
+  moreover have "?f (g a') \<in> A'" if a': "a' \<in> A'" for a'
+  proof -
+    let ?phi = "\<lambda> b'. b' \<in> A' \<and> g b' = g a'"
+    from a' have "?phi a'" by auto
+    then have "?phi (SOME b'. ?phi b')"
+      using someI[of ?phi] by blast
+    then show ?thesis by (auto simp: inv_into_def)
+  qed
+  ultimately show "\<exists>f. inj_on f (g ` A') \<and> f ` g ` A' \<subseteq> A'"
+    by auto
 qed
 
 lemma Ex_inj_on_UNION_Sigma:
   "\<exists>f. (inj_on f (\<Union>i \<in> I. A i) \<and> f ` (\<Union>i \<in> I. A i) \<le> (SIGMA i : I. A i))"
 proof
-  let ?phi = "\<lambda> a i. i \<in> I \<and> a \<in> A i"
-  let ?sm = "\<lambda> a. SOME i. ?phi a i"
+  let ?phi = "\<lambda>a i. i \<in> I \<and> a \<in> A i"
+  let ?sm = "\<lambda>a. SOME i. ?phi a i"
   let ?f = "\<lambda>a. (?sm a, a)"
-  have "inj_on ?f (\<Union>i \<in> I. A i)" unfolding inj_on_def by auto
+  have "inj_on ?f (\<Union>i \<in> I. A i)"
+    by (auto simp: inj_on_def)
   moreover
-  { { fix i a assume "i \<in> I" and "a \<in> A i"
-      hence "?sm a \<in> I \<and> a \<in> A(?sm a)" using someI[of "?phi a" i] by auto
-    }
-    hence "?f ` (\<Union>i \<in> I. A i) \<le> (SIGMA i : I. A i)" by auto
-  }
-  ultimately
-  show "inj_on ?f (\<Union>i \<in> I. A i) \<and> ?f ` (\<Union>i \<in> I. A i) \<le> (SIGMA i : I. A i)"
-  by auto
+  have "?sm a \<in> I \<and> a \<in> A(?sm a)" if "i \<in> I" and "a \<in> A i" for i a
+    using that someI[of "?phi a" i] by auto
+  then have "?f ` (\<Union>i \<in> I. A i) \<le> (SIGMA i : I. A i)"
+    by auto
+  ultimately show "inj_on ?f (\<Union>i \<in> I. A i) \<and> ?f ` (\<Union>i \<in> I. A i) \<le> (SIGMA i : I. A i)"
+    by auto
 qed
 
 lemma inv_unique_comp:
@@ -448,190 +455,199 @@ lemma inv_unique_comp:
 subsection \<open>The Cantor-Bernstein Theorem\<close>
 
 lemma Cantor_Bernstein_aux:
-  shows "\<exists>A' h. A' \<le> A \<and>
-                (\<forall>a \<in> A'. a \<notin> g`(B - f ` A')) \<and>
-                (\<forall>a \<in> A'. h a = f a) \<and>
-                (\<forall>a \<in> A - A'. h a \<in> B - (f ` A') \<and> a = g(h a))"
-proof-
-  obtain H where H_def: "H = (\<lambda> A'. A - (g`(B - (f ` A'))))" by blast
-  have 0: "mono H" unfolding mono_def H_def by blast
-  then obtain A' where 1: "H A' = A'" using lfp_unfold by blast
-  hence 2: "A' = A - (g`(B - (f ` A')))" unfolding H_def by simp
-  hence 3: "A' \<le> A" by blast
-  have 4: "\<forall>a \<in> A'.  a \<notin> g`(B - f ` A')"
-  using 2 by blast
-  have 5: "\<forall>a \<in> A - A'. \<exists>b \<in> B - (f ` A'). a = g b"
-  using 2 by blast
-  (*  *)
-  obtain h where h_def:
-  "h = (\<lambda> a. if a \<in> A' then f a else (SOME b. b \<in> B - (f ` A') \<and> a = g b))" by blast
-  hence "\<forall>a \<in> A'. h a = f a" by auto
-  moreover
-  have "\<forall>a \<in> A - A'. h a \<in> B - (f ` A') \<and> a = g(h a)"
+  "\<exists>A' h. A' \<subseteq> A \<and>
+    (\<forall>a \<in> A'. a \<notin> g ` (B - f ` A')) \<and>
+    (\<forall>a \<in> A'. h a = f a) \<and>
+    (\<forall>a \<in> A - A'. h a \<in> B - (f ` A') \<and> a = g (h a))"
+proof -
+  define H where "H A' = A - (g ` (B - (f ` A')))" for A'
+  have "mono H" unfolding mono_def H_def by blast
+  from lfp_unfold [OF this] obtain A' where "H A' = A'" by blast
+  then have "A' = A - (g ` (B - (f ` A')))" by (simp add: H_def)
+  then have 1: "A' \<subseteq> A"
+    and 2: "\<forall>a \<in> A'.  a \<notin> g ` (B - f ` A')"
+    and 3: "\<forall>a \<in> A - A'. \<exists>b \<in> B - (f ` A'). a = g b"
+    by blast+
+  define h where "h a = (if a \<in> A' then f a else (SOME b. b \<in> B - (f ` A') \<and> a = g b))" for a
+  then have 4: "\<forall>a \<in> A'. h a = f a" by simp
+  have "\<forall>a \<in> A - A'. h a \<in> B - (f ` A') \<and> a = g (h a)"
   proof
-    fix a assume *: "a \<in> A - A'"
-    let ?phi = "\<lambda> b. b \<in> B - (f ` A') \<and> a = g b"
-    have "h a = (SOME b. ?phi b)" using h_def * by auto
-    moreover have "\<exists>b. ?phi b" using 5 *  by auto
-    ultimately show  "?phi (h a)" using someI_ex[of ?phi] by auto
+    fix a
+    let ?phi = "\<lambda>b. b \<in> B - (f ` A') \<and> a = g b"
+    assume *: "a \<in> A - A'"
+    from * have "h a = (SOME b. ?phi b)" by (auto simp: h_def)
+    moreover from 3 * have "\<exists>b. ?phi b" by auto
+    ultimately show "?phi (h a)"
+      using someI_ex[of ?phi] by auto
   qed
-  ultimately show ?thesis using 3 4 by blast
+  with 1 2 4 show ?thesis by blast
 qed
 
 theorem Cantor_Bernstein:
-  assumes INJ1: "inj_on f A" and SUB1: "f ` A \<le> B" and
-          INJ2: "inj_on g B" and SUB2: "g ` B \<le> A"
+  assumes inj1: "inj_on f A" and sub1: "f ` A \<subseteq> B"
+    and inj2: "inj_on g B" and sub2: "g ` B \<subseteq> A"
   shows "\<exists>h. bij_betw h A B"
 proof-
-  obtain A' and h where 0: "A' \<le> A" and
-  1: "\<forall>a \<in> A'. a \<notin> g`(B - f ` A')" and
-  2: "\<forall>a \<in> A'. h a = f a" and
-  3: "\<forall>a \<in> A - A'. h a \<in> B - (f ` A') \<and> a = g(h a)"
-  using Cantor_Bernstein_aux[of A g B f] by blast
+  obtain A' and h where "A' \<subseteq> A"
+    and 1: "\<forall>a \<in> A'. a \<notin> g ` (B - f ` A')"
+    and 2: "\<forall>a \<in> A'. h a = f a"
+    and 3: "\<forall>a \<in> A - A'. h a \<in> B - (f ` A') \<and> a = g (h a)"
+    using Cantor_Bernstein_aux [of A g B f] by blast
   have "inj_on h A"
   proof (intro inj_onI)
     fix a1 a2
     assume 4: "a1 \<in> A" and 5: "a2 \<in> A" and 6: "h a1 = h a2"
     show "a1 = a2"
-    proof(cases "a1 \<in> A'")
-      assume Case1: "a1 \<in> A'"
+    proof (cases "a1 \<in> A'")
+      case True
       show ?thesis
-      proof(cases "a2 \<in> A'")
-        assume Case11: "a2 \<in> A'"
-        hence "f a1 = f a2" using Case1 2 6 by auto
-        thus ?thesis using INJ1 Case1 Case11 0
-        unfolding inj_on_def by blast
+      proof (cases "a2 \<in> A'")
+        case True': True
+        with True 2 6 have "f a1 = f a2" by auto
+        with inj1 \<open>A' \<subseteq> A\<close> True True' show ?thesis
+          unfolding inj_on_def by blast
       next
-        assume Case12: "a2 \<notin> A'"
-        hence False using 3 5 2 6 Case1 by force
-        thus ?thesis by simp
+        case False
+        with 2 3 5 6 True have False by force
+        then show ?thesis ..
       qed
     next
-    assume Case2: "a1 \<notin> A'"
+      case False
       show ?thesis
-      proof(cases "a2 \<in> A'")
-        assume Case21: "a2 \<in> A'"
-        hence False using 3 4 2 6 Case2 by auto
-        thus ?thesis by simp
+      proof (cases "a2 \<in> A'")
+        case True
+        with 2 3 4 6 False have False by auto
+        then show ?thesis ..
       next
-        assume Case22: "a2 \<notin> A'"
-        hence "a1 = g(h a1) \<and> a2 = g(h a2)" using Case2 4 5 3 by auto
-        thus ?thesis using 6 by simp
+        case False': False
+        with False 3 4 5 have "a1 = g (h a1)" "a2 = g (h a2)" by auto
+        with 6 show ?thesis by simp
       qed
     qed
   qed
-  (*  *)
-  moreover
-  have "h ` A = B"
+  moreover have "h ` A = B"
   proof safe
-    fix a assume "a \<in> A"
-    thus "h a \<in> B" using SUB1 2 3 by (cases "a \<in> A'") auto
+    fix a
+    assume "a \<in> A"
+    with sub1 2 3 show "h a \<in> B" by (cases "a \<in> A'") auto
   next
-    fix b assume *: "b \<in> B"
+    fix b
+    assume *: "b \<in> B"
     show "b \<in> h ` A"
-    proof(cases "b \<in> f ` A'")
-      assume Case1: "b \<in> f ` A'"
-      then obtain a where "a \<in> A' \<and> b = f a" by blast
-      thus ?thesis using 2 0 by force
+    proof (cases "b \<in> f ` A'")
+      case True
+      then obtain a where "a \<in> A'" "b = f a" by blast
+      with \<open>A' \<subseteq> A\<close> 2 show ?thesis by force
     next
-      assume Case2: "b \<notin> f ` A'"
-      hence "g b \<notin> A'" using 1 * by auto
-      hence 4: "g b \<in> A - A'" using * SUB2 by auto
-      hence "h(g b) \<in> B \<and> g(h(g b)) = g b"
-      using 3 by auto
-      hence "h(g b) = b" using * INJ2 unfolding inj_on_def by auto
-      thus ?thesis using 4 by force
+      case False
+      with 1 * have "g b \<notin> A'" by auto
+      with sub2 * have 4: "g b \<in> A - A'" by auto
+      with 3 have "h (g b) \<in> B" "g (h (g b)) = g b" by auto
+      with inj2 * have "h (g b) = b" by (auto simp: inj_on_def)
+      with 4 show ?thesis by force
     qed
   qed
-  (*  *)
-  ultimately show ?thesis unfolding bij_betw_def by auto
+  ultimately show ?thesis
+    by (auto simp: bij_betw_def)
 qed
+
 
 subsection \<open>Other Consequences of Hilbert's Epsilon\<close>
 
 text \<open>Hilbert's Epsilon and the @{term split} Operator\<close>
 
-text\<open>Looping simprule\<close>
-lemma split_paired_Eps: "(SOME x. P x) = (SOME (a,b). P(a,b))"
+text \<open>Looping simprule!\<close>
+lemma split_paired_Eps: "(SOME x. P x) = (SOME (a, b). P (a, b))"
   by simp
 
 lemma Eps_case_prod: "Eps (case_prod P) = (SOME xy. P (fst xy) (snd xy))"
   by (simp add: split_def)
 
-lemma Eps_case_prod_eq [simp]: "(@(x',y'). x = x' & y = y') = (x,y)"
+lemma Eps_case_prod_eq [simp]: "(SOME (x', y'). x = x' \<and> y = y') = (x, y)"
   by blast
 
 
-text\<open>A relation is wellfounded iff it has no infinite descending chain\<close>
-lemma wf_iff_no_infinite_down_chain:
-  "wf r = (~(\<exists>f. \<forall>i. (f(Suc i),f i) \<in> r))"
-apply (simp only: wf_eq_minimal)
-apply (rule iffI)
- apply (rule notI)
- apply (erule exE)
- apply (erule_tac x = "{w. \<exists>i. w=f i}" in allE, blast)
-apply (erule contrapos_np, simp, clarify)
-apply (subgoal_tac "\<forall>n. rec_nat x (%i y. @z. z:Q & (z,y) :r) n \<in> Q")
- apply (rule_tac x = "rec_nat x (%i y. @z. z:Q & (z,y) :r)" in exI)
- apply (rule allI, simp)
- apply (rule someI2_ex, blast, blast)
-apply (rule allI)
-apply (induct_tac "n", simp_all)
-apply (rule someI2_ex, blast+)
-done
+text \<open>A relation is wellfounded iff it has no infinite descending chain.\<close>
+lemma wf_iff_no_infinite_down_chain: "wf r \<longleftrightarrow> (\<not> (\<exists>f. \<forall>i. (f (Suc i), f i) \<in> r))"
+  apply (simp only: wf_eq_minimal)
+  apply (rule iffI)
+   apply (rule notI)
+   apply (erule exE)
+   apply (erule_tac x = "{w. \<exists>i. w = f i}" in allE)
+   apply blast
+  apply (erule contrapos_np)
+  apply simp
+  apply clarify
+  apply (subgoal_tac "\<forall>n. rec_nat x (\<lambda>i y. SOME z. z \<in> Q \<and> (z, y) \<in> r) n \<in> Q")
+   apply (rule_tac x = "rec_nat x (\<lambda>i y. SOME z. z \<in> Q \<and> (z, y) \<in> r)" in exI)
+   apply (rule allI)
+   apply simp
+   apply (rule someI2_ex)
+    apply blast
+   apply blast
+  apply (rule allI)
+  apply (induct_tac n)
+   apply simp_all
+  apply (rule someI2_ex)
+   apply blast
+  apply blast
+  done
 
 lemma wf_no_infinite_down_chainE:
-  assumes "wf r" obtains k where "(f (Suc k), f k) \<notin> r"
-using \<open>wf r\<close> wf_iff_no_infinite_down_chain[of r] by blast
+  assumes "wf r"
+  obtains k where "(f (Suc k), f k) \<notin> r"
+  using assms wf_iff_no_infinite_down_chain[of r] by blast
 
 
-text\<open>A dynamically-scoped fact for TFL\<close>
-lemma tfl_some: "\<forall>P x. P x --> P (Eps P)"
+text \<open>A dynamically-scoped fact for TFL\<close>
+lemma tfl_some: "\<forall>P x. P x \<longrightarrow> P (Eps P)"
   by (blast intro: someI)
 
 
 subsection \<open>Least value operator\<close>
 
-definition
-  LeastM :: "['a => 'b::ord, 'a => bool] => 'a" where
-  "LeastM m P == SOME x. P x & (\<forall>y. P y --> m x <= m y)"
+definition LeastM :: "('a \<Rightarrow> 'b::ord) \<Rightarrow> ('a \<Rightarrow> bool) \<Rightarrow> 'a"
+  where "LeastM m P \<equiv> (SOME x. P x \<and> (\<forall>y. P y \<longrightarrow> m x \<le> m y))"
 
 syntax
-  "_LeastM" :: "[pttrn, 'a => 'b::ord, bool] => 'a"    ("LEAST _ WRT _. _" [0, 4, 10] 10)
+  "_LeastM" :: "pttrn \<Rightarrow> ('a \<Rightarrow> 'b::ord) \<Rightarrow> bool \<Rightarrow> 'a"  ("LEAST _ WRT _. _" [0, 4, 10] 10)
 translations
-  "LEAST x WRT m. P" == "CONST LeastM m (%x. P)"
+  "LEAST x WRT m. P" \<rightleftharpoons> "CONST LeastM m (\<lambda>x. P)"
 
 lemma LeastMI2:
-  "P x ==> (!!y. P y ==> m x <= m y)
-    ==> (!!x. P x ==> \<forall>y. P y --> m x \<le> m y ==> Q x)
-    ==> Q (LeastM m P)"
+  "P x \<Longrightarrow>
+    (\<And>y. P y \<Longrightarrow> m x \<le> m y) \<Longrightarrow>
+    (\<And>x. P x \<Longrightarrow> \<forall>y. P y \<longrightarrow> m x \<le> m y \<Longrightarrow> Q x) \<Longrightarrow>
+    Q (LeastM m P)"
   apply (simp add: LeastM_def)
-  apply (rule someI2_ex, blast, blast)
+  apply (rule someI2_ex)
+   apply blast
+  apply blast
   done
 
 lemma LeastM_equality:
-  "P k ==> (!!x. P x ==> m k <= m x)
-    ==> m (LEAST x WRT m. P x) = (m k::'a::order)"
-  apply (rule LeastMI2, assumption, blast)
+  "P k \<Longrightarrow> (\<And>x. P x \<Longrightarrow> m k \<le> m x) \<Longrightarrow> m (LEAST x WRT m. P x) = (m k :: 'a::order)"
+  apply (rule LeastMI2)
+    apply assumption
+   apply blast
   apply (blast intro!: order_antisym)
   done
 
 lemma wf_linord_ex_has_least:
-  "wf r ==> \<forall>x y. ((x,y):r^+) = ((y,x)~:r^*) ==> P k
-    ==> \<exists>x. P x & (!y. P y --> (m x,m y):r^*)"
+  "wf r \<Longrightarrow> \<forall>x y. (x, y) \<in> r\<^sup>+ \<longleftrightarrow> (y, x) \<notin> r\<^sup>* \<Longrightarrow> P k \<Longrightarrow> \<exists>x. P x \<and> (\<forall>y. P y \<longrightarrow> (m x, m y) \<in> r\<^sup>*)"
   apply (drule wf_trancl [THEN wf_eq_minimal [THEN iffD1]])
-  apply (drule_tac x = "m`Collect P" in spec, force)
+  apply (drule_tac x = "m ` Collect P" in spec)
+  apply force
   done
 
-lemma ex_has_least_nat:
-    "P k ==> \<exists>x. P x & (\<forall>y. P y --> m x <= (m y::nat))"
+lemma ex_has_least_nat: "P k \<Longrightarrow> \<exists>x. P x \<and> (\<forall>y. P y \<longrightarrow> m x \<le> (m y :: nat))"
   apply (simp only: pred_nat_trancl_eq_le [symmetric])
   apply (rule wf_pred_nat [THEN wf_linord_ex_has_least])
-   apply (simp add: less_eq linorder_not_le pred_nat_trancl_eq_le, assumption)
+   apply (simp add: less_eq linorder_not_le pred_nat_trancl_eq_le)
+  apply assumption
   done
 
-lemma LeastM_nat_lemma:
-    "P k ==> P (LeastM m P) & (\<forall>y. P y --> m (LeastM m P) <= (m y::nat))"
+lemma LeastM_nat_lemma: "P k \<Longrightarrow> P (LeastM m P) \<and> (\<forall>y. P y \<longrightarrow> m (LeastM m P) \<le> (m y :: nat))"
   apply (simp add: LeastM_def)
   apply (rule someI_ex)
   apply (erule ex_has_least_nat)
@@ -639,91 +655,87 @@ lemma LeastM_nat_lemma:
 
 lemmas LeastM_natI = LeastM_nat_lemma [THEN conjunct1]
 
-lemma LeastM_nat_le: "P x ==> m (LeastM m P) <= (m x::nat)"
-by (rule LeastM_nat_lemma [THEN conjunct2, THEN spec, THEN mp], assumption, assumption)
+lemma LeastM_nat_le: "P x \<Longrightarrow> m (LeastM m P) \<le> (m x :: nat)"
+  by (rule LeastM_nat_lemma [THEN conjunct2, THEN spec, THEN mp])
 
 
 subsection \<open>Greatest value operator\<close>
 
-definition
-  GreatestM :: "['a => 'b::ord, 'a => bool] => 'a" where
-  "GreatestM m P == SOME x. P x & (\<forall>y. P y --> m y <= m x)"
+definition GreatestM :: "('a \<Rightarrow> 'b::ord) \<Rightarrow> ('a \<Rightarrow> bool) \<Rightarrow> 'a"
+  where "GreatestM m P \<equiv> SOME x. P x \<and> (\<forall>y. P y \<longrightarrow> m y \<le> m x)"
 
-definition
-  Greatest :: "('a::ord => bool) => 'a" (binder "GREATEST " 10) where
-  "Greatest == GreatestM (%x. x)"
+definition Greatest :: "('a::ord \<Rightarrow> bool) \<Rightarrow> 'a"  (binder "GREATEST " 10)
+  where "Greatest \<equiv> GreatestM (\<lambda>x. x)"
 
 syntax
-  "_GreatestM" :: "[pttrn, 'a => 'b::ord, bool] => 'a"
-      ("GREATEST _ WRT _. _" [0, 4, 10] 10)
+  "_GreatestM" :: "pttrn \<Rightarrow> ('a \<Rightarrow> 'b::ord) \<Rightarrow> bool \<Rightarrow> 'a"  ("GREATEST _ WRT _. _" [0, 4, 10] 10)
 translations
-  "GREATEST x WRT m. P" == "CONST GreatestM m (%x. P)"
+  "GREATEST x WRT m. P" \<rightleftharpoons> "CONST GreatestM m (\<lambda>x. P)"
 
 lemma GreatestMI2:
-  "P x ==> (!!y. P y ==> m y <= m x)
-    ==> (!!x. P x ==> \<forall>y. P y --> m y \<le> m x ==> Q x)
-    ==> Q (GreatestM m P)"
+  "P x \<Longrightarrow>
+    (\<And>y. P y \<Longrightarrow> m y \<le> m x) \<Longrightarrow>
+    (\<And>x. P x \<Longrightarrow> \<forall>y. P y \<longrightarrow> m y \<le> m x \<Longrightarrow> Q x) \<Longrightarrow>
+    Q (GreatestM m P)"
   apply (simp add: GreatestM_def)
-  apply (rule someI2_ex, blast, blast)
+  apply (rule someI2_ex)
+   apply blast
+  apply blast
   done
 
 lemma GreatestM_equality:
- "P k ==> (!!x. P x ==> m x <= m k)
-    ==> m (GREATEST x WRT m. P x) = (m k::'a::order)"
-  apply (rule_tac m = m in GreatestMI2, assumption, blast)
+  "P k \<Longrightarrow>
+    (\<And>x. P x \<Longrightarrow> m x \<le> m k) \<Longrightarrow>
+    m (GREATEST x WRT m. P x) = (m k :: 'a::order)"
+  apply (rule GreatestMI2 [where m = m])
+    apply assumption
+   apply blast
   apply (blast intro!: order_antisym)
   done
 
-lemma Greatest_equality:
-  "P (k::'a::order) ==> (!!x. P x ==> x <= k) ==> (GREATEST x. P x) = k"
+lemma Greatest_equality: "P k \<Longrightarrow> (\<And>x. P x \<Longrightarrow> x \<le> k) \<Longrightarrow> (GREATEST x. P x) = k"
+  for k :: "'a::order"
   apply (simp add: Greatest_def)
-  apply (erule GreatestM_equality, blast)
+  apply (erule GreatestM_equality)
+  apply blast
   done
 
 lemma ex_has_greatest_nat_lemma:
-  "P k ==> \<forall>x. P x --> (\<exists>y. P y & ~ ((m y::nat) <= m x))
-    ==> \<exists>y. P y & ~ (m y < m k + n)"
-  apply (induct n, force)
-  apply (force simp add: le_Suc_eq)
-  done
+  "P k \<Longrightarrow> \<forall>x. P x \<longrightarrow> (\<exists>y. P y \<and> \<not> m y \<le> (m x :: nat)) \<Longrightarrow> \<exists>y. P y \<and> \<not> m y < m k + n"
+  by (induct n) (force simp: le_Suc_eq)+
 
 lemma ex_has_greatest_nat:
-  "P k ==> \<forall>y. P y --> m y < b
-    ==> \<exists>x. P x & (\<forall>y. P y --> (m y::nat) <= m x)"
+  "P k \<Longrightarrow> \<forall>y. P y \<longrightarrow> m y < b \<Longrightarrow> \<exists>x. P x \<and> (\<forall>y. P y \<longrightarrow> m y \<le> (m x :: nat))"
   apply (rule ccontr)
   apply (cut_tac P = P and n = "b - m k" in ex_has_greatest_nat_lemma)
-    apply (subgoal_tac [3] "m k <= b", auto)
+    apply (subgoal_tac [3] "m k \<le> b")
+     apply auto
   done
 
 lemma GreatestM_nat_lemma:
-  "P k ==> \<forall>y. P y --> m y < b
-    ==> P (GreatestM m P) & (\<forall>y. P y --> (m y::nat) <= m (GreatestM m P))"
+  "P k \<Longrightarrow> \<forall>y. P y \<longrightarrow> m y < b \<Longrightarrow>
+    P (GreatestM m P) \<and> (\<forall>y. P y \<longrightarrow> (m y :: nat) \<le> m (GreatestM m P))"
   apply (simp add: GreatestM_def)
   apply (rule someI_ex)
-  apply (erule ex_has_greatest_nat, assumption)
+  apply (erule ex_has_greatest_nat)
+  apply assumption
   done
 
 lemmas GreatestM_natI = GreatestM_nat_lemma [THEN conjunct1]
 
-lemma GreatestM_nat_le:
-  "P x ==> \<forall>y. P y --> m y < b
-    ==> (m x::nat) <= m (GreatestM m P)"
-  apply (blast dest: GreatestM_nat_lemma [THEN conjunct2, THEN spec, of P])
-  done
+lemma GreatestM_nat_le: "P x \<Longrightarrow> \<forall>y. P y \<longrightarrow> m y < b \<Longrightarrow> (m x :: nat) \<le> m (GreatestM m P)"
+  by (blast dest: GreatestM_nat_lemma [THEN conjunct2, THEN spec, of P])
 
 
-text \<open>\medskip Specialization to \<open>GREATEST\<close>.\<close>
+text \<open>\<^medskip> Specialization to \<open>GREATEST\<close>.\<close>
 
-lemma GreatestI: "P (k::nat) ==> \<forall>y. P y --> y < b ==> P (GREATEST x. P x)"
-  apply (simp add: Greatest_def)
-  apply (rule GreatestM_natI, auto)
-  done
+lemma GreatestI: "P k \<Longrightarrow> \<forall>y. P y \<longrightarrow> y < b \<Longrightarrow> P (GREATEST x. P x)"
+  for k :: nat
+  unfolding Greatest_def by (rule GreatestM_natI) auto
 
-lemma Greatest_le:
-    "P x ==> \<forall>y. P y --> y < b ==> (x::nat) <= (GREATEST x. P x)"
-  apply (simp add: Greatest_def)
-  apply (rule GreatestM_nat_le, auto)
-  done
+lemma Greatest_le: "P x \<Longrightarrow> \<forall>y. P y \<longrightarrow> y < b \<Longrightarrow> x \<le> (GREATEST x. P x)"
+  for x :: nat
+  unfolding Greatest_def by (rule GreatestM_nat_le) auto
 
 
 subsection \<open>An aside: bounded accessible part\<close>
@@ -732,7 +744,8 @@ text \<open>Finite monotone eventually stable sequences\<close>
 
 lemma finite_mono_remains_stable_implies_strict_prefix:
   fixes f :: "nat \<Rightarrow> 'a::order"
-  assumes S: "finite (range f)" "mono f" and eq: "\<forall>n. f n = f (Suc n) \<longrightarrow> f (Suc n) = f (Suc (Suc n))"
+  assumes S: "finite (range f)" "mono f"
+    and eq: "\<forall>n. f n = f (Suc n) \<longrightarrow> f (Suc n) = f (Suc (Suc n))"
   shows "\<exists>N. (\<forall>n\<le>N. \<forall>m\<le>N. m < n \<longrightarrow> f m < f n) \<and> (\<forall>n\<ge>N. f N = f n)"
   using assms
 proof -
@@ -740,15 +753,16 @@ proof -
   proof (rule ccontr)
     assume "\<not> ?thesis"
     then have "\<And>n. f n \<noteq> f (Suc n)" by auto
-    then have "\<And>n. f n < f (Suc n)"
-      using  \<open>mono f\<close> by (auto simp: le_less mono_iff_le_Suc)
-    with lift_Suc_mono_less_iff[of f]
-    have *: "\<And>n m. n < m \<Longrightarrow> f n < f m" by auto
+    with \<open>mono f\<close> have "\<And>n. f n < f (Suc n)"
+      by (auto simp: le_less mono_iff_le_Suc)
+    with lift_Suc_mono_less_iff[of f] have *: "\<And>n m. n < m \<Longrightarrow> f n < f m"
+      by auto
     have "inj f"
     proof (intro injI)
       fix x y
       assume "f x = f y"
-      then show "x = y" by (cases x y rule: linorder_cases) (auto dest: *)
+      then show "x = y"
+        by (cases x y rule: linorder_cases) (auto dest: *)
     qed
     with \<open>finite (range f)\<close> have "finite (UNIV::nat set)"
       by (rule finite_imageD)
@@ -760,16 +774,22 @@ proof -
     unfolding N_def using n by (rule LeastI)
   show ?thesis
   proof (intro exI[of _ N] conjI allI impI)
-    fix n assume "N \<le> n"
+    fix n
+    assume "N \<le> n"
     then have "\<And>m. N \<le> m \<Longrightarrow> m \<le> n \<Longrightarrow> f m = f N"
     proof (induct rule: dec_induct)
-      case (step n) then show ?case
-        using eq[rule_format, of "n - 1"] N
+      case base
+      then show ?case by simp
+    next
+      case (step n)
+      then show ?case
+        using eq [rule_format, of "n - 1"] N
         by (cases n) (auto simp add: le_Suc_eq)
-    qed simp
+    qed
     from this[of n] \<open>N \<le> n\<close> show "f N = f n" by auto
   next
-    fix n m :: nat assume "m < n" "n \<le> N"
+    fix n m :: nat
+    assume "m < n" "n \<le> N"
     then show "f m < f n"
     proof (induct rule: less_Suc_induct)
       case (1 i)
@@ -777,37 +797,41 @@ proof -
       then have "f i \<noteq> f (Suc i)"
         unfolding N_def by (rule not_less_Least)
       with \<open>mono f\<close> show ?case by (simp add: mono_iff_le_Suc less_le)
-    qed auto
+    next
+      case 2
+      then show ?case by simp
+    qed
   qed
 qed
 
 lemma finite_mono_strict_prefix_implies_finite_fixpoint:
   fixes f :: "nat \<Rightarrow> 'a set"
   assumes S: "\<And>i. f i \<subseteq> S" "finite S"
-    and inj: "\<exists>N. (\<forall>n\<le>N. \<forall>m\<le>N. m < n \<longrightarrow> f m \<subset> f n) \<and> (\<forall>n\<ge>N. f N = f n)"
+    and ex: "\<exists>N. (\<forall>n\<le>N. \<forall>m\<le>N. m < n \<longrightarrow> f m \<subset> f n) \<and> (\<forall>n\<ge>N. f N = f n)"
   shows "f (card S) = (\<Union>n. f n)"
 proof -
-  from inj obtain N where inj: "(\<forall>n\<le>N. \<forall>m\<le>N. m < n \<longrightarrow> f m \<subset> f n)" and eq: "(\<forall>n\<ge>N. f N = f n)" by auto
-
-  { fix i have "i \<le> N \<Longrightarrow> i \<le> card (f i)"
-    proof (induct i)
-      case 0 then show ?case by simp
-    next
-      case (Suc i)
-      with inj[rule_format, of "Suc i" i]
-      have "(f i) \<subset> (f (Suc i))" by auto
-      moreover have "finite (f (Suc i))" using S by (rule finite_subset)
-      ultimately have "card (f i) < card (f (Suc i))" by (intro psubset_card_mono)
-      with Suc show ?case using inj by auto
-    qed
-  }
+  from ex obtain N where inj: "\<And>n m. n \<le> N \<Longrightarrow> m \<le> N \<Longrightarrow> m < n \<Longrightarrow> f m \<subset> f n"
+    and eq: "\<forall>n\<ge>N. f N = f n"
+    by atomize auto
+  have "i \<le> N \<Longrightarrow> i \<le> card (f i)" for i
+  proof (induct i)
+    case 0
+    then show ?case by simp
+  next
+    case (Suc i)
+    with inj [of "Suc i" i] have "(f i) \<subset> (f (Suc i))" by auto
+    moreover have "finite (f (Suc i))" using S by (rule finite_subset)
+    ultimately have "card (f i) < card (f (Suc i))" by (intro psubset_card_mono)
+    with Suc inj show ?case by auto
+  qed
   then have "N \<le> card (f N)" by simp
   also have "\<dots> \<le> card S" using S by (intro card_mono)
   finally have "f (card S) = f N" using eq by auto
-  then show ?thesis using eq inj[rule_format, of N]
+  then show ?thesis
+    using eq inj [of N]
     apply auto
     apply (case_tac "n < N")
-    apply (auto simp: not_less)
+     apply (auto simp: not_less)
     done
 qed
 
@@ -819,183 +843,174 @@ locale bijection =
   assumes bij: "bij f"
 begin
 
-lemma bij_inv:
-  "bij (inv f)"
+lemma bij_inv: "bij (inv f)"
   using bij by (rule bij_imp_bij_inv)
 
-lemma surj [simp]:
-  "surj f"
+lemma surj [simp]: "surj f"
   using bij by (rule bij_is_surj)
 
-lemma inj:
-  "inj f"
+lemma inj: "inj f"
   using bij by (rule bij_is_inj)
 
-lemma surj_inv [simp]:
-  "surj (inv f)"
+lemma surj_inv [simp]: "surj (inv f)"
   using inj by (rule inj_imp_surj_inv)
 
-lemma inj_inv:
-  "inj (inv f)"
+lemma inj_inv: "inj (inv f)"
   using surj by (rule surj_imp_inj_inv)
 
-lemma eqI:
-  "f a = f b \<Longrightarrow> a = b"
+lemma eqI: "f a = f b \<Longrightarrow> a = b"
   using inj by (rule injD)
 
-lemma eq_iff [simp]:
-  "f a = f b \<longleftrightarrow> a = b"
+lemma eq_iff [simp]: "f a = f b \<longleftrightarrow> a = b"
   by (auto intro: eqI)
 
-lemma eq_invI:
-  "inv f a = inv f b \<Longrightarrow> a = b"
+lemma eq_invI: "inv f a = inv f b \<Longrightarrow> a = b"
   using inj_inv by (rule injD)
 
-lemma eq_inv_iff [simp]:
-  "inv f a = inv f b \<longleftrightarrow> a = b"
+lemma eq_inv_iff [simp]: "inv f a = inv f b \<longleftrightarrow> a = b"
   by (auto intro: eq_invI)
 
-lemma inv_left [simp]:
-  "inv f (f a) = a"
+lemma inv_left [simp]: "inv f (f a) = a"
   using inj by (simp add: inv_f_eq)
 
-lemma inv_comp_left [simp]:
-  "inv f \<circ> f = id"
+lemma inv_comp_left [simp]: "inv f \<circ> f = id"
   by (simp add: fun_eq_iff)
 
-lemma inv_right [simp]:
-  "f (inv f a) = a"
+lemma inv_right [simp]: "f (inv f a) = a"
   using surj by (simp add: surj_f_inv_f)
 
-lemma inv_comp_right [simp]:
-  "f \<circ> inv f = id"
+lemma inv_comp_right [simp]: "f \<circ> inv f = id"
   by (simp add: fun_eq_iff)
 
-lemma inv_left_eq_iff [simp]:
-  "inv f a = b \<longleftrightarrow> f b = a"
+lemma inv_left_eq_iff [simp]: "inv f a = b \<longleftrightarrow> f b = a"
   by auto
 
-lemma inv_right_eq_iff [simp]:
-  "b = inv f a \<longleftrightarrow> f b = a"
+lemma inv_right_eq_iff [simp]: "b = inv f a \<longleftrightarrow> f b = a"
   by auto
 
 end
 
 lemma infinite_imp_bij_betw:
-assumes INF: "\<not> finite A"
-shows "\<exists>h. bij_betw h A (A - {a})"
-proof(cases "a \<in> A")
-  assume Case1: "a \<notin> A"  hence "A - {a} = A" by blast
-  thus ?thesis using bij_betw_id[of A] by auto
+  assumes infinite: "\<not> finite A"
+  shows "\<exists>h. bij_betw h A (A - {a})"
+proof (cases "a \<in> A")
+  case False
+  then have "A - {a} = A" by blast
+  then show ?thesis
+    using bij_betw_id[of A] by auto
 next
-  assume Case2: "a \<in> A"
-  have "\<not> finite (A - {a})" using INF by auto
-  with infinite_iff_countable_subset[of "A - {a}"] obtain f::"nat \<Rightarrow> 'a"
-  where 1: "inj f" and 2: "f ` UNIV \<le> A - {a}" by blast
-  obtain g where g_def: "g = (\<lambda> n. if n = 0 then a else f (Suc n))" by blast
-  obtain A' where A'_def: "A' = g ` UNIV" by blast
-  have temp: "\<forall>y. f y \<noteq> a" using 2 by blast
-  have 3: "inj_on g UNIV \<and> g ` UNIV \<le> A \<and> a \<in> g ` UNIV"
-  proof(auto simp add: Case2 g_def, unfold inj_on_def, intro ballI impI,
-        case_tac "x = 0", auto simp add: 2)
-    fix y  assume "a = (if y = 0 then a else f (Suc y))"
-    thus "y = 0" using temp by (case_tac "y = 0", auto)
+  case True
+  with infinite have "\<not> finite (A - {a})" by auto
+  with infinite_iff_countable_subset[of "A - {a}"]
+  obtain f :: "nat \<Rightarrow> 'a" where 1: "inj f" and 2: "f ` UNIV \<subseteq> A - {a}" by blast
+  define g where "g n = (if n = 0 then a else f (Suc n))" for n
+  define A' where "A' = g ` UNIV"
+  have *: "\<forall>y. f y \<noteq> a" using 2 by blast
+  have 3: "inj_on g UNIV \<and> g ` UNIV \<subseteq> A \<and> a \<in> g ` UNIV"
+    apply (auto simp add: True g_def [abs_def])
+     apply (unfold inj_on_def)
+     apply (intro ballI impI)
+     apply (case_tac "x = 0")
+      apply (auto simp add: 2)
+  proof -
+    fix y
+    assume "a = (if y = 0 then a else f (Suc y))"
+    then show "y = 0" by (cases "y = 0") (use * in auto)
   next
     fix x y
     assume "f (Suc x) = (if y = 0 then a else f (Suc y))"
-    thus "x = y" using 1 temp unfolding inj_on_def by (case_tac "y = 0", auto)
+    with 1 * show "x = y" by (cases "y = 0") (auto simp: inj_on_def)
   next
-    fix n show "f (Suc n) \<in> A" using 2 by blast
+    fix n
+    from 2 show "f (Suc n) \<in> A" by blast
   qed
-  hence 4: "bij_betw g UNIV A' \<and> a \<in> A' \<and> A' \<le> A"
-  using inj_on_imp_bij_betw[of g] unfolding A'_def by auto
-  hence 5: "bij_betw (inv g) A' UNIV"
-  by (auto simp add: bij_betw_inv_into)
-  (*  *)
-  obtain n where "g n = a" using 3 by auto
-  hence 6: "bij_betw g (UNIV - {n}) (A' - {a})"
-  using 3 4 unfolding A'_def
-  by clarify (rule bij_betw_subset, auto simp: image_set_diff)
-  (*  *)
-  obtain v where v_def: "v = (\<lambda> m. if m < n then m else Suc m)" by blast
+  then have 4: "bij_betw g UNIV A' \<and> a \<in> A' \<and> A' \<subseteq> A"
+    using inj_on_imp_bij_betw[of g] by (auto simp: A'_def)
+  then have 5: "bij_betw (inv g) A' UNIV"
+    by (auto simp add: bij_betw_inv_into)
+  from 3 obtain n where n: "g n = a" by auto
+  have 6: "bij_betw g (UNIV - {n}) (A' - {a})"
+    by (rule bij_betw_subset) (use 3 4 n in \<open>auto simp: image_set_diff A'_def\<close>)
+  define v where "v m = (if m < n then m else Suc m)" for m
   have 7: "bij_betw v UNIV (UNIV - {n})"
-  proof(unfold bij_betw_def inj_on_def, intro conjI, clarify)
-    fix m1 m2 assume "v m1 = v m2"
-    thus "m1 = m2"
-    by(case_tac "m1 < n", case_tac "m2 < n",
-       auto simp add: inj_on_def v_def, case_tac "m2 < n", auto)
+  proof (unfold bij_betw_def inj_on_def, intro conjI, clarify)
+    fix m1 m2
+    assume "v m1 = v m2"
+    then show "m1 = m2"
+      apply (cases "m1 < n")
+       apply (cases "m2 < n")
+        apply (auto simp: inj_on_def v_def [abs_def])
+      apply (cases "m2 < n")
+       apply auto
+      done
   next
     show "v ` UNIV = UNIV - {n}"
-    proof(auto simp add: v_def)
-      fix m assume *: "m \<noteq> n" and **: "m \<notin> Suc ` {m'. \<not> m' < n}"
-      {assume "n \<le> m" with * have 71: "Suc n \<le> m" by auto
-       then obtain m' where 72: "m = Suc m'" using Suc_le_D by auto
-       with 71 have "n \<le> m'" by auto
-       with 72 ** have False by auto
-      }
-      thus "m < n" by force
+    proof (auto simp: v_def [abs_def])
+      fix m
+      assume "m \<noteq> n"
+      assume *: "m \<notin> Suc ` {m'. \<not> m' < n}"
+      have False if "n \<le> m"
+      proof -
+        from \<open>m \<noteq> n\<close> that have **: "Suc n \<le> m" by auto
+        from Suc_le_D [OF this] obtain m' where m': "m = Suc m'" ..
+        with ** have "n \<le> m'" by auto
+        with m' * show ?thesis by auto
+      qed
+      then show "m < n" by force
     qed
   qed
-  (*  *)
-  obtain h' where h'_def: "h' = g o v o (inv g)" by blast
-  hence 8: "bij_betw h' A' (A' - {a})" using 5 7 6
-  by (auto simp add: bij_betw_trans)
-  (*  *)
-  obtain h where h_def: "h = (\<lambda> b. if b \<in> A' then h' b else b)" by blast
-  have "\<forall>b \<in> A'. h b = h' b" unfolding h_def by auto
-  hence "bij_betw h  A' (A' - {a})" using 8 bij_betw_cong[of A' h] by auto
+  define h' where "h' = g \<circ> v \<circ> (inv g)"
+  with 5 6 7 have 8: "bij_betw h' A' (A' - {a})"
+    by (auto simp add: bij_betw_trans)
+  define h where "h b = (if b \<in> A' then h' b else b)" for b
+  then have "\<forall>b \<in> A'. h b = h' b" by simp
+  with 8 have "bij_betw h  A' (A' - {a})"
+    using bij_betw_cong[of A' h] by auto
   moreover
-  {have "\<forall>b \<in> A - A'. h b = b" unfolding h_def by auto
-   hence "bij_betw h  (A - A') (A - A')"
-   using bij_betw_cong[of "A - A'" h id] bij_betw_id[of "A - A'"] by auto
-  }
+  have "\<forall>b \<in> A - A'. h b = b" by (auto simp: h_def)
+  then have "bij_betw h  (A - A') (A - A')"
+    using bij_betw_cong[of "A - A'" h id] bij_betw_id[of "A - A'"] by auto
   moreover
-  have "(A' Int (A - A') = {} \<and> A' \<union> (A - A') = A) \<and>
-        ((A' - {a}) Int (A - A') = {} \<and> (A' - {a}) \<union> (A - A') = A - {a})"
-  using 4 by blast
+  from 4 have "(A' \<inter> (A - A') = {} \<and> A' \<union> (A - A') = A) \<and>
+    ((A' - {a}) \<inter> (A - A') = {} \<and> (A' - {a}) \<union> (A - A') = A - {a})"
+    by blast
   ultimately have "bij_betw h A (A - {a})"
-  using bij_betw_combine[of h A' "A' - {a}" "A - A'" "A - A'"] by simp
-  thus ?thesis by blast
+    using bij_betw_combine[of h A' "A' - {a}" "A - A'" "A - A'"] by simp
+  then show ?thesis by blast
 qed
 
 lemma infinite_imp_bij_betw2:
-assumes INF: "\<not> finite A"
-shows "\<exists>h. bij_betw h A (A \<union> {a})"
-proof(cases "a \<in> A")
-  assume Case1: "a \<in> A"  hence "A \<union> {a} = A" by blast
-  thus ?thesis using bij_betw_id[of A] by auto
+  assumes "\<not> finite A"
+  shows "\<exists>h. bij_betw h A (A \<union> {a})"
+proof (cases "a \<in> A")
+  case True
+  then have "A \<union> {a} = A" by blast
+  then show ?thesis using bij_betw_id[of A] by auto
 next
+  case False
   let ?A' = "A \<union> {a}"
-  assume Case2: "a \<notin> A" hence "A = ?A' - {a}" by blast
-  moreover have "\<not> finite ?A'" using INF by auto
+  from False have "A = ?A' - {a}" by blast
+  moreover from assms have "\<not> finite ?A'" by auto
   ultimately obtain f where "bij_betw f ?A' A"
-  using infinite_imp_bij_betw[of ?A' a] by auto
-  hence "bij_betw(inv_into ?A' f) A ?A'" using bij_betw_inv_into by blast
-  thus ?thesis by auto
+    using infinite_imp_bij_betw[of ?A' a] by auto
+  then have "bij_betw (inv_into ?A' f) A ?A'" by (rule bij_betw_inv_into)
+  then show ?thesis by auto
 qed
 
-lemma bij_betw_inv_into_left:
-assumes BIJ: "bij_betw f A A'" and IN: "a \<in> A"
-shows "(inv_into A f) (f a) = a"
-using assms unfolding bij_betw_def
-by clarify (rule inv_into_f_f)
+lemma bij_betw_inv_into_left: "bij_betw f A A' \<Longrightarrow> a \<in> A \<Longrightarrow> inv_into A f (f a) = a"
+  unfolding bij_betw_def by clarify (rule inv_into_f_f)
 
-lemma bij_betw_inv_into_right:
-assumes "bij_betw f A A'" "a' \<in> A'"
-shows "f(inv_into A f a') = a'"
-using assms unfolding bij_betw_def using f_inv_into_f by force
+lemma bij_betw_inv_into_right: "bij_betw f A A' \<Longrightarrow> a' \<in> A' \<Longrightarrow> f (inv_into A f a') = a'"
+  unfolding bij_betw_def using f_inv_into_f by force
 
 lemma bij_betw_inv_into_subset:
-assumes BIJ: "bij_betw f A A'" and
-        SUB: "B \<le> A" and IM: "f ` B = B'"
-shows "bij_betw (inv_into A f) B' B"
-using assms unfolding bij_betw_def
-by (auto intro: inj_on_inv_into)
+  "bij_betw f A A' \<Longrightarrow> B \<subseteq> A \<Longrightarrow> f ` B = B' \<Longrightarrow> bij_betw (inv_into A f) B' B"
+  by (auto simp: bij_betw_def intro: inj_on_inv_into)
 
 
 subsection \<open>Specification package -- Hilbertized version\<close>
 
-lemma exE_some: "[| Ex P ; c == Eps P |] ==> P c"
+lemma exE_some: "Ex P \<Longrightarrow> c \<equiv> Eps P \<Longrightarrow> P c"
   by (simp only: someI_ex)
 
 ML_file "Tools/choice_specification.ML"
